updates

Veritas.Hash.fsti
@@ -11,3 +11,6 @@ type hash_value = bv_t hash_size
 
 (* hash function maps a merkle payload to a hash value *)
 val hashfn (v:value): Tot hash_value
+
+type hash_collision = 
+  | Collision: v1:value -> v2:value {hashfn v1 = hashfn v2 /\ ~(v1 = v2)} -> hash_collision
