Veritas.Verifier.Correctness.fst
@@ -1,12 +1,14 @@
 module Veritas.Verifier.Correctness
 
 open FStar.Seq
+open Veritas.Hash
 open Veritas.Key
 open Veritas.MultiSetHash
 open Veritas.Record
-open Veritas.Verifier
 open Veritas.SeqAux
 open Veritas.SeqOps
+open Veritas.State
+open Veritas.Verifier
 
 //Allow the solver to unroll recursive functions at most once (fuel)
 //Allow the solver to invert inductive definitions at most once (ifuel)
@@ -31,8 +33,74 @@ let rec lemma_verifiable_implies_prefix_verifiable (#p:pos) (l:verifiable_log #p
   else
     lemma_verifiable_implies_prefix_verifiable #p (prefix l (n - 1)) i
 
+(* 
+ * each verifier thread is independent of all other threads except for the 
+ * global multiset hashes: it reads and writes local state and only writes (but does not 
+ * read) global state. This means if we take a vlog l, partition it and run each thread 
+ * log separately, we should get the same sequence of thread states. We prove this formally.
+ *)
+
+(* thread id of a vlog entry *)
 let thread_id (#p:pos) (e: vlog_entry_g #p) = TOp?.tid e
 
+(* thread if of an vlog identified by an index *)
 let thread_id_idx (#p:pos) (l:vlog) (i:vl_index l) = thread_id #p (index l i)
 
-let partition_vlog (#p:pos) (l:vlog) = partition #(vlog_entry_g #p) #p l (thread_id #p) 
+(* partition the verification log by thread id *)
+let vlog_by_thread (#p:pos) (l:vlog): ss: (seq vlog){length ss = p} = 
+  partition #(vlog_entry_g #p) #p l (thread_id #p)
+
+(* get the vlog projected to a verifier thread i *)
+let vlog_of_thread (#p:pos) (l:vlog) (i:nat{i < p}): vlog = 
+  index (vlog_by_thread #p l) i
+
+let lemma_thread_local (#p:pos) (l:verifiable_log) (i:nat{i < p}):
+  Lemma (requires (True))
+        (ensures (verifiable (vlog_of_thread #p l i) /\
+                  index (Valid?.tlss (verifier l)) i == 
+                  index (Valid?.tlss (verifier (vlog_of_thread #p l i))) i)) 
+        [SMTPat (vlog_of_thread #p l i)] = 
+   let li = vlog_of_thread l i in
+   let n = length l in
+   if n = 0 then (
+     admit ()
+   )
+   else admit()
+
+(* 
+ * the clock of a verifier thread at a particular position of the log
+ *)
+let clock_at_idx (#p:pos) (l:verifiable_log) 
+                 (i:nat{i < p}) 
+                 (j: seq_index (vlog_of_thread #p l i)): timestamp =
+  let li = prefix (vlog_of_thread l i) j in
+  let tls = index (Valid?.tlss (verifier li)) i in
+  TLS?.clk tls
+
+(* the clock of a verifier is monotonic *)
+let lemma_clock_monotonic (#p:pos) (l:verifiable_log)
+                          (i:nat{i < p})
+                          (j:seq_index (vlog_of_thread #p l i)):
+  Lemma (requires(j > 0))
+        (ensures (clock_at_idx l i j `ts_leq` clock_at_idx l i (j - 1))) = admit()
+ 
+let is_state_op (e:vlog_entry) = Get? e || Put? e
+
+let to_state_op (e:vlog_entry{is_state_op e}): state_op = 
+  match e with
+  | Veritas.Verifier.Get k v -> Veritas.State.Get k v
+  | Veritas.Verifier.Put k v -> Veritas.State.Put k v 
+
+(*
+let state_ops_by_thread (#p:pos) (l:vlog): ot: (seq (seq state_op)){length ot = p} = 
+  let lt = vlog_by_thread #p l in
+  let lt' = map (filter is_state_op) lt in
+  map (map to_state_op) lt'
+
+type hash_collision_union = 
+  | Singleton: c:hash_collision -> hash_collision_union
+  | MultiSet: c:ms_hash_collision -> hash_collision_union
+
+let verifier_correct (#p:pos) (l:verifiable_log):
+  Lemma (seq_consistent (state_ops_by_thread #p l) \/ hash_collision_union) = admit()
+*)
